aneris/examples/snapshot_isolation/examples/no_serializability/no_serializability_proof.v
@@ -63,8 +63,9 @@ Local Open Scope list.
     iIntros (cst sa) "#inv %Φ !>(CanStart & #HiC) HΦ".
     rewrite/transaction1.
     wp_pures.
-    wp_apply (SI_start_spec $! _ _ (⊤ ∖ ↑client_inv_name));
+    wp_apply (SI_start_spec _ _ (⊤ ∖ ↑client_inv_name));
       first solve_ndisj.
+    iFrame "#".
     iInv "inv" as ">(%hx & %hy & %hz & x_hx & y_hy & z_hz & init)" "close".
     iModIntro.
     iExists {[ "x" := hx; "y" := hy; "z" := hz ]}.
@@ -87,19 +88,23 @@ Local Open Scope list.
       first done.
     iPoseProof (big_sepM_insert with "cache") as "((z_hz & z_upd) & _)";
       first done.
-    wp_apply (SI_write_spec $! _ _ _ _ (SerVal #1) with "[] [$x_hx $x_upd $HiC]");
+    wp_apply (SI_write_spec _ _ _ _ (SerVal #1)
+               with "[] [$] [$x_hx $x_upd $HiC]");
       first set_solver.
     iIntros "(x_1 & x_upd)".
     wp_pures.
-    wp_apply (SI_write_spec $! _ _ _ _ (SerVal #1) with "[] [$y_hy $y_upd $HiC]");
+    wp_apply (SI_write_spec _ _ _ _ (SerVal #1)
+               with "[] [$] [$y_hy $y_upd $HiC]");
       first set_solver.
     iIntros "(y_1 & y_upd)".
     wp_pures.
-    wp_apply (SI_write_spec $! _ _ _ _ (SerVal #1) with "[] [$z_hz $z_upd $HiC]");
+    wp_apply (SI_write_spec _ _ _ _ (SerVal #1)
+               with "[] [$] [$z_hz $z_upd $HiC]");
       first set_solver.
     iIntros "(z_1 & z_upd)".
     wp_pures.
-    wp_apply (commitU_spec _ _ (⊤ ∖ ↑client_inv_name)); first solve_ndisj.
+    wp_apply (commitU_spec _ _ (⊤ ∖ ↑client_inv_name));
+      first solve_ndisj; eauto.
     iInv "inv" as ">(%hx' & %hy' & %hz' & x_hx' & y_hy' & z_hz' & #init)" "close".
     iModIntro.
     iExists {[ "x" := hx'; "y" := hy'; "z" := hz' ]}, _,
@@ -153,16 +158,17 @@ Local Open Scope list.
 
   Lemma transaction2_spec :
     ∀ cst sa,
-    client_inv -∗
+      client_inv -∗
+      GlobalInv -∗
     {{{ ConnectionState cst sa CanStart ∗ IsConnected cst sa }}}
       transaction2 cst @[ip_of_address sa]
     {{{ RET #(); True }}}.
   Proof.
-    iIntros (cst sa) "#inv %Φ !>(CanStart & #HiC) HΦ".
+    iIntros (cst sa) "#inv #Hginv %Φ !>(CanStart & #HiC) HΦ".
     rewrite/transaction2.
     wp_pures.
     wp_apply (simple_wait_transaction_spec _ _ _ _ _  (⊤ ∖ ↑client_inv_name)
-      with "[] [] [] [] [$CanStart $HiC]"); [solve_ndisj|set_solver|..].
+      with "[] [] [$] [] [] [$CanStart]"); [solve_ndisj|set_solver|..].
     {
       iModIntro.
       iInv "inv" as ">(%hx & %hy & %hz & x_hx & y_hy & z_hz & %Hinv)" "close".
@@ -184,11 +190,11 @@ Local Open Scope list.
     }
     iIntros (h) "(CanStart & #Seen)".
     wp_pures.
-    wp_apply (SI_start_spec $! _ _ (⊤ ∖ ↑client_inv_name)); first solve_ndisj.
+    wp_apply (SI_start_spec _ _ (⊤ ∖ ↑client_inv_name)); first solve_ndisj; eauto.
     iInv "inv" as ">(%hx & %hy & %hz & x_hx & y_hy & z_hz &
       [->|(%vx & %vy & %hx_vx & %hy_vy & %Hvx & %Hvy)])" "close".
     {
-      iMod (Seen_valid $! SI_GlobalInv with "[$Seen $z_hz]") as
+      iMod (Seen_valid with "[$][$Seen $z_hz]") as
           "(z_hz & %abs)"; first solve_ndisj.
       apply prefix_nil_inv in abs.
       by apply app_nil in abs as [_].
@@ -215,19 +221,21 @@ Local Open Scope list.
         "((x_hx & x_upd) & cache)"; first done.
     iPoseProof (big_sepM_delete _ _ "y" hy with "cache") as
         "((y_hy & y_upd) & cache)"; first by rewrite lookup_delete_ne.
-    wp_apply (SI_read_spec with "[] [ $HiC $x_hx]"); first set_solver.
+    wp_apply (SI_read_spec with "[][][$x_hx]");
+      first set_solver; eauto.
     iIntros "x_hx".
     rewrite hx_vx hy_vy.
     destruct Hvx as [-> | ->].
     all: wp_pures.
-    wp_apply (SI_write_spec $! _ _ _ _ (SerVal #(-1)) with
-        "[] [$y_hy $y_upd  $HiC]"); first set_solver.
+    wp_apply (SI_write_spec _ _ _ _ (SerVal #(-1)) with
+        "[][][$y_hy $y_upd]"); first set_solver; eauto.
     iIntros "(y_hy & y_upd)".
     wp_pures.
-    all: wp_apply (commitU_spec _ _ (⊤ ∖ ↑client_inv_name)); first solve_ndisj.
+    all: wp_apply (commitU_spec _ _ (⊤ ∖ ↑client_inv_name));
+      first solve_ndisj; eauto.
     all: iInv "inv" as ">(%hx' & %hy' & %hz' & x_hx' & y_hy' & z_hz' &
       [->|(%vx' & %vy' & %hx'_vx' & %hy'_vy' & %Hvx' & %Hvy')])" "close".
-    1, 3: iMod (Seen_valid $! SI_GlobalInv with "[$Seen $z_hz']") as
+    1, 3: iMod (Seen_valid with "[$][$Seen $z_hz']") as
             "(z_hz' & %abs)"; first solve_ndisj.
     1, 2:  apply prefix_nil_inv in abs.
     by apply app_nil in abs as [_].
@@ -267,16 +275,18 @@ Local Open Scope list.
 
   Lemma transaction3_spec :
     ∀ cst sa,
-    client_inv -∗
+     client_inv -∗
+     GlobalInv -∗
     {{{ ConnectionState cst sa CanStart ∗ IsConnected cst sa }}}
       transaction3 cst @[ip_of_address sa]
     {{{ RET #(); True }}}.
   Proof.
-    iIntros (cst sa) "#inv %Φ!>(CanStart & #HiC) HΦ".
+    iIntros (cst sa) "#inv #Hginv %Φ!>(CanStart & #HiC) HΦ".
     rewrite/transaction3.
     wp_pures.
     wp_apply (simple_wait_transaction_spec _ _ _ _ _ (⊤ ∖ ↑client_inv_name)
-      with "[] [] [] [] [$CanStart $HiC]"); [solve_ndisj|set_solver|..].
+               with "[] [] [] [] [] [$CanStart $HiC]");
+      try eauto; [solve_ndisj |..].
     {
       iModIntro.
       iInv "inv" as ">(%hx & %hy & %hz & x_hx & y_hy & z_hz & %Hinv)" "close".
@@ -298,12 +308,12 @@ Local Open Scope list.
     }
     iIntros (h) "(CanStart & #Seen)".
     wp_pures.
-    wp_apply (SI_start_spec $! _ _ (⊤ ∖ ↑client_inv_name)); first solve_ndisj.
+    wp_apply (SI_start_spec _ _ (⊤ ∖ ↑client_inv_name)); first solve_ndisj; eauto.
     iInv "inv" as ">(%hx & %hy & %hz & x_hx & y_hy & z_hz &
       [->|(%vx & %vy & %hx_vx & %hy_vy & %Hvx & %Hvy)])" "close".
     {
-      iMod (Seen_valid $! SI_GlobalInv with "[$Seen $z_hz]") as
-          "(z_hz & %abs)"; first solve_ndisj.
+      iMod (Seen_valid with "[$][$Seen $z_hz]") as
+          "(z_hz & %abs)"; first solve_ndisj; eauto.
        apply prefix_nil_inv in abs.
     by apply app_nil in abs as [_].
     }
@@ -329,19 +339,20 @@ Local Open Scope list.
         "((x_hx & x_upd) & cache)"; first done.
     iPoseProof (big_sepM_delete _ _ "y" hy with "cache") as
         "((y_hy & y_upd) & _)"; first by rewrite lookup_delete_ne.
-    wp_apply (SI_read_spec with "[] [$y_hy $HiC]"); first set_solver.
+    wp_apply (SI_read_spec with "[][$][$y_hy]"); first set_solver.
     iIntros "y_hy".
     rewrite hx_vx hy_vy.
     destruct Hvy as [-> | ->].
     all: wp_pures.
-    wp_apply (SI_write_spec $! _ _ _ _ (SerVal #(-1)) with
-        "[] [$x_hx $x_upd $HiC]"); first set_solver.
+    wp_apply (SI_write_spec _ _ _ _ (SerVal #(-1)) with
+        "[][$][$x_hx $x_upd]"); first set_solver.
     iIntros "(x_hx & x_upd)".
     wp_pures.
-    all: wp_apply (commitU_spec _ _ (⊤ ∖ ↑client_inv_name)); first solve_ndisj.
+    all: wp_apply (commitU_spec _ _ (⊤ ∖ ↑client_inv_name));
+      first solve_ndisj; eauto.
     all: iInv "inv" as ">(%hx' & %hy' & %hz' & x_hx' & y_hy' & z_hz' &
       [->|(%vx' & %vy' & %hx'_vx' & %hy'_vy' & %Hvx' & %Hvy')])" "close".
-    1, 3: iMod (Seen_valid $! SI_GlobalInv with "[$Seen $z_hz']") as
+    1, 3: iMod (Seen_valid with "[$][$Seen $z_hz']") as
             "(z_hz' & %abs)"; first solve_ndisj.
     1, 2:  apply prefix_nil_inv in abs.
     by apply app_nil in abs as [_].
@@ -381,16 +392,17 @@ Local Open Scope list.
 
   Lemma transaction4_spec :
     ∀ cst sa,
-    client_inv -∗
+      client_inv -∗
+      GlobalInv -∗
     {{{ ConnectionState cst sa CanStart ∗ IsConnected cst sa }}}
       transaction4 cst @[ip_of_address sa]
     {{{ RET #(); True }}}.
   Proof.
-    iIntros (cst sa) "#inv %Φ !>(CanStart & #HiC) HΦ".
+    iIntros (cst sa) "#inv #Hgivn %Φ !>(CanStart & #HiC) HΦ".
     rewrite/transaction4.
     wp_pures.
     wp_apply (simple_wait_transaction_spec _ _ _ _ _ (⊤ ∖ ↑client_inv_name)
-      with "[] [] [] [] [$CanStart $HiC]"); [solve_ndisj|set_solver|..].
+      with "[] [] [$] [] [] [$CanStart]"); [solve_ndisj|set_solver|..].
     {
       iModIntro.
       iInv "inv" as ">(%hx & %hy & %hz & x_hx & y_hy & z_hz & %Hinv)" "close".
@@ -412,11 +424,11 @@ Local Open Scope list.
     }
     iIntros (h) "(CanStart & #Seen)".
     wp_pures.
-    wp_apply (SI_start_spec $! _ _ (⊤ ∖ ↑client_inv_name)); first solve_ndisj.
+    wp_apply (SI_start_spec _ _ (⊤ ∖ ↑client_inv_name)); first solve_ndisj; eauto.
     iInv "inv" as ">(%hx & %hy & %hz & x_hx & y_hy & z_hz &
       [->|(%vx & %vy & %hx_vx & %hy_vy & %Hvx & %Hvy)])" "close".
     {
-      iMod (Seen_valid $! SI_GlobalInv with "[$Seen $z_hz]") as
+      iMod (Seen_valid with "[$][$Seen $z_hz]") as
           "(z_hz & %abs)"; first solve_ndisj.
        apply prefix_nil_inv in abs.
     by apply app_nil in abs as [_].
@@ -443,16 +455,16 @@ Local Open Scope list.
         "((x_hx & x_upd) & cache)"; first done.
     iPoseProof (big_sepM_delete _ _ "y" hy with "cache") as
         "((y_hy & y_upd) & _)"; first by rewrite lookup_delete_ne.
-    wp_apply (SI_read_spec with "[]  [$x_hx $HiC]"); first set_solver.
+    wp_apply (SI_read_spec with "[] [$] [$x_hx $HiC]"); first set_solver.
     iIntros "x_hx".
     rewrite hx_vx hy_vy/unSOME /assert.
     wp_pures.
-    wp_apply (SI_read_spec with "[] [$y_hy $HiC]"); first set_solver.
+    wp_apply (SI_read_spec with "[][$] [$y_hy $HiC]"); first set_solver.
     iIntros "y_hy".
     wp_pures.
     move: Hvx Hvy hx_vx hy_vy=>[]->[]->hx_vx hy_vy.
     all: wp_pures.
-    all: wp_apply (commitU_spec _ _ (⊤ ∖ ↑client_inv_name)); first solve_ndisj.
+    all: wp_apply (commitU_spec _ _ (⊤ ∖ ↑client_inv_name)); first solve_ndisj; eauto.
     all: iInv "inv" as ">(%hx' & %hy' & %hz' & x_hx' & y_hy' & z_hz' & %Hinv)"
                           "close".
     all: iModIntro.
@@ -504,6 +516,7 @@ Local Open Scope list.
 
   Lemma transaction2_client_spec :
     ∀ sa,
+    GlobalInv -∗
     client_inv -∗
     {{{
       sa ⤳ (∅, ∅) ∗
@@ -515,18 +528,19 @@ Local Open Scope list.
       transaction2_client $sa $KVS_address @[ip_of_address sa]
     {{{ RET #(); True }}}.
   Proof.
-    iIntros (sa) "#inv %Φ !>(∅ & unalloc & free & Hcc & #KVS_si) HΦ".
+    iIntros (sa) "#Hginv #inv %Φ !>(∅ & unalloc & free & Hcc & #KVS_si) HΦ".
     rewrite/transaction2_client.
     wp_pures.
     wp_apply (SI_init_client_proxy_spec with "[$]").
     iIntros (cst) "CanStart".
     wp_pures.
-    by wp_apply (transaction2_spec with "inv [$]").
+    by wp_apply (transaction2_spec with "[$inv] [$] [$]").
   Qed.
 
   Lemma transaction3_client_spec :
     ∀ sa,
-    client_inv -∗
+      client_inv -∗
+      GlobalInv -∗
     {{{
       sa ⤳ (∅, ∅) ∗
       unallocated {[sa]} ∗
@@ -537,18 +551,19 @@ Local Open Scope list.
       transaction3_client $sa $KVS_address @[ip_of_address sa]
     {{{ RET #(); True }}}.
   Proof.
-    iIntros (sa) "#inv %Φ !>(∅ & unalloc & free & Hcc & #KVS_si) HΦ".
+    iIntros (sa) "#inv #Hginv %Φ !>(∅ & unalloc & free & Hcc & #KVS_si) HΦ".
     rewrite/transaction3_client.
     wp_pures.
     wp_apply (SI_init_client_proxy_spec with "[$]").
     iIntros (cst) "CanStart".
     wp_pures.
-    by wp_apply (transaction3_spec with "inv [$]").
+    by wp_apply (transaction3_spec with "inv [$] [$]").
   Qed.
 
   Lemma transaction4_client_spec :
     ∀ sa,
-    client_inv -∗
+      client_inv -∗
+      GlobalInv -∗
     {{{
       sa ⤳ (∅, ∅) ∗
       unallocated {[sa]} ∗
@@ -559,13 +574,14 @@ Local Open Scope list.
       transaction4_client $sa $KVS_address @[ip_of_address sa]
     {{{ RET #(); True }}}.
   Proof.
-    iIntros (sa) "#inv %Φ !>(∅ & unalloc & Hcc & free & #KVS_si) HΦ".
+    iIntros (sa)
+      "#inv #Hginv %Φ !>(∅ & unalloc & Hcc & free & #KVS_si) HΦ".
     rewrite/transaction4_client.
     wp_pures.
     wp_apply (SI_init_client_proxy_spec with "[$]").
     iIntros (cst) "CanStart".
     wp_pures.
-    by wp_apply (transaction4_spec with "inv [$]").
+    by wp_apply (transaction4_spec with "inv [$][$]").
   Qed.
 
   Lemma server_spec :
@@ -623,7 +639,8 @@ Context `{!anerisG Mdl Σ, !SI_init, !KVSG Σ}.
             _
             {[client_1_addr; client_2_addr;
               client_3_addr; client_4_addr]})
-      as (SI_res SI_client_toolbox) "(mem & KVS_Init & Hcc)".
+      as (SI_res) "(mem & KVS_Init & #Hginv & Hcc & %specs)".
+    destruct specs as (Hs1 & Hs2 & Hs3 & Hs4 & Hs5 & Hs6).
     iPoseProof (big_sepS_delete _ _ "x" with "mem") as "(mem_x & mem)";
       first done.
     iPoseProof (big_sepS_delete _ _ "y" with "mem") as "(mem_y & mem)";
@@ -675,7 +692,8 @@ Context `{!anerisG Mdl Σ, !SI_init, !KVSG Σ}.
     iSplitR "clt2_∅ clt2_unalloc Hcc2"; last first.
     {
       iIntros "!>Hports".
-      by wp_apply (transaction2_client_spec client_2_addr with "inv [$]").
+      by wp_apply (transaction2_client_spec client_2_addr
+             with "Hginv inv [$]").
     }
     iNext.
     wp_pures.
@@ -684,7 +702,8 @@ Context `{!anerisG Mdl Σ, !SI_init, !KVSG Σ}.
     iSplitR "clt3_∅ clt3_unalloc Hcc3"; last first.
     {
       iIntros "!>Hports".
-      by wp_apply (transaction3_client_spec client_3_addr with "inv [$]").
+      by wp_apply (transaction3_client_spec client_3_addr
+             with "inv Hginv [$]").
     }
     iNext.
     wp_pures.
@@ -693,9 +712,11 @@ Context `{!anerisG Mdl Σ, !SI_init, !KVSG Σ}.
     iSplitR "clt4_∅ clt4_unalloc Hcc4"; last first.
     {
       iIntros "!>Hports".
-      by wp_apply (transaction4_client_spec client_4_addr with "inv [$]").
+      by wp_apply (transaction4_client_spec client_4_addr with
+             "inv Hginv  [$]").
     }
     by iApply "HΦ".
+    Unshelve. all: by eauto.
   Qed.
 
 End proof_runner.
