aneris/examples/snapshot_isolation/instantiation/instantiation_of_init.v
@@ -1,10 +1,32 @@
+From iris.algebra Require Import agree auth excl gmap updates local_updates.
+From iris.algebra.lib Require Import mono_list.
+From iris.base_logic.lib Require Import mono_nat ghost_map.
+From iris.base_logic Require Import invariants.
+From iris.bi.lib Require Import fractional.
+From iris.proofmode Require Import tactics.
+From aneris.prelude Require Import list.
+From aneris.algebra Require Import monotone.
+From aneris.aneris_lang Require Import lang resources resources inject.
+From aneris.lib Require Import gen_heap_light.
+From aneris.aneris_lang.lib Require Import
+     list_proof lock_proof map_proof.
+From aneris.aneris_lang.lib.serialization Require Import
+  serialization_proof.
 From aneris.examples.snapshot_isolation
      Require Import snapshot_isolation_code
                     snapshot_isolation_code_api.
 From aneris.aneris_lang Require Import resources.
-From aneris.examples.snapshot_isolation.specs Require Import user_params specs.
-From aneris.examples.snapshot_isolation.instantiation
-     Require Import snapshot_isolation_api_implementation.
+From aneris.examples.reliable_communication.lib.mt_server Require Import user_params.
+From aneris.examples.snapshot_isolation.specs Require Import
+  user_params resources specs.
+From aneris.examples.snapshot_isolation.proof.resources Require Import
+  resource_algebras
+  global_invariant.
+From aneris.examples.snapshot_isolation.instantiation Require Import
+  snapshot_isolation_api_implementation
+  instantiation_of_resources.
+From aneris.examples.snapshot_isolation.proof.server Require Import
+  proof_of_init_server.
 
 Global Instance SI_init_instanciation `{!anerisG Mdl Σ, !User_params} :
     SI_init.
