aneris/examples/snapshot_isolation/instantiation/snapshot_isolation_api_implementation.v
@@ -2,7 +2,8 @@ From aneris.examples.snapshot_isolation
      Require Import snapshot_isolation_code
                     snapshot_isolation_code_api.
 From aneris.aneris_lang Require Import resources.
-From aneris.examples.snapshot_isolation.specs Require Import user_params specs.
+From aneris.examples.snapshot_isolation.specs Require Import
+  user_params.
 
 Global Instance KVS_snapshot_isolation_api_implementation :
         KVS_snapshot_isolation_api :=
